Sitpn/SitpnComplete.v
@@ -1,0 +1,83 @@
+(* Import Sitpn material. *)
+
+Require Import Hilecop.Sitpn.Sitpn.
+Require Import Hilecop.Sitpn.SitpnTokenPlayer.
+Require Import Hilecop.Sitpn.SitpnSemantics.
+
+(* Import falling edge and rising edge completeness lemmas. *)
+
+Require Import Hilecop.Sitpn.SitpnFallingEdgeComplete.
+Require Import Hilecop.Sitpn.SitpnRisingEdgeComplete.
+
+(* Import lemmas on SITPN and states well-definition. *)
+
+Require Import Hilecop.Sitpn.SitpnFallingEdgeWellDef.
+
+(** * Completeness proof between [sitpn_cycle] and [SitpnSemantics]. *)
+
+Theorem sitpn_cycle_complete :
+  forall (sitpn : Sitpn)
+         (s s' s'' : SitpnState)
+         (time_value : nat)
+         (env : Condition -> nat -> bool),
+    IsWellDefinedSitpn sitpn ->
+    IsWellDefinedSitpnState sitpn s ->
+    IsWellDefinedSitpnState sitpn s' ->
+    IsWellDefinedSitpnState sitpn s'' ->
+    SitpnSemantics sitpn s s' time_value env falling_edge ->
+    SitpnSemantics sitpn s' s'' time_value env rising_edge ->
+    exists (istate fstate : SitpnState),
+      sitpn_cycle sitpn s time_value env = Some (istate, fstate) /\
+      sitpn_state_eq s' istate /\
+      sitpn_state_eq s'' fstate.
+Proof.
+  intros sitpn s s' s'' t env
+         Hwell_def_sitpn Hwell_def_s Hwell_def_s' Hwell_def_s''
+         Hfall_spec Hrising_spec.
+
+  (* Let's dig the function!! *)
+  unfold sitpn_cycle.
+
+  (* Specializes sitpn_falling_edge_complete then rewrites the goal *)
+  specialize (sitpn_falling_edge_complete
+                sitpn s s' t env Hwell_def_sitpn
+                Hwell_def_s Hwell_def_s' Hfall_spec)
+    as Hex_fall_fun.
+  inversion_clear Hex_fall_fun as (istate & Hw_fall_fun).
+  inversion_clear Hw_fall_fun as (Hfall_fun & Hsteq_s'_istate).
+  rewrite Hfall_fun.
+  
+  (* Specializes sitpn_rising_no_error, then rewrites the goal. 
+     Cannot directly rewrite the goal by specializing sitpn_rising_edge_complete. *)
+
+  (* Builds premise IsWellDefinedSitpnState sitpn inter_state 
+     to specialize sitpn_rising_edge_no_error. *)
+  specialize (sitpn_falling_edge_well_def_state
+                sitpn s istate t env Hwell_def_sitpn Hwell_def_s Hfall_fun)
+    as Hwell_def_istate.
+  specialize (sitpn_rising_edge_no_error sitpn istate Hwell_def_sitpn Hwell_def_istate)
+    as Hex_rising_fun_noerr.
+  inversion_clear Hex_rising_fun_noerr as (fstate & Hrising_fun_noerr).
+  rewrite Hrising_fun_noerr.
+  
+  (* Specializes sitpn_rising_edge_complete, then shows
+     that the fstate and fs verify the sitpn_state_eq relation. *)
+
+  specialize (sitpn_rising_edge_complete
+                sitpn s' s'' t env Hwell_def_sitpn Hwell_def_s'
+                Hwell_def_s'' Hrising_spec)
+    as Hex_rising_fun.
+  inversion_clear Hex_rising_fun as (fs & Hw_rising_fun).
+  inversion_clear Hw_rising_fun as (Hrising_fun & Hsteq_s''_fs).
+
+  specialize (sitpn_rising_edge_state_eq
+                sitpn s' fs istate fstate Hsteq_s'_istate
+                Hrising_fun Hrising_fun_noerr)
+    as Hsteq_fs_fstate.
+  
+  (* Instantiates states, and proves the goal. *)
+  exists istate, fstate.
+  split; [reflexivity |
+          split; [ assumption | rewrite <- Hsteq_fs_fstate; assumption]
+         ].  
+Qed.
