Sitpn/SitpnFallingEdgeComplete.v
@@ -1,0 +1,21 @@
+(* Import Sitpn material. *)
+
+Require Import Hilecop.Sitpn.Sitpn.
+Require Import Hilecop.Sitpn.SitpnTokenPlayer.
+Require Import Hilecop.Sitpn.SitpnSemantics.
+
+(** * Completeness of [sitpn_falling_edge]. *)
+
+Lemma sitpn_falling_edge_complete :
+  forall (sitpn : Sitpn)
+         (s s' : SitpnState)
+         (time_value : nat)
+         (env : Condition -> nat -> bool),
+    IsWellDefinedSitpn sitpn ->
+    IsWellDefinedSitpnState sitpn s ->
+    IsWellDefinedSitpnState sitpn s' ->
+    SitpnSemantics sitpn s s' time_value env falling_edge ->
+    exists istate : SitpnState,
+      sitpn_falling_edge sitpn s time_value env = Some istate /\
+      sitpn_state_eq s' istate.
+Admitted.
