Sitpn/SitpnRisingEdgeStateEq.v
@@ -1,0 +1,220 @@
+(* Import Sitpn material. *)
+
+Require Import Hilecop.Sitpn.Sitpn.
+Require Import Hilecop.Sitpn.SitpnTokenPlayer.
+Require Import Hilecop.Sitpn.SitpnSemantics.
+
+(* Import lemmas on fired transitions. *)
+
+Require Import Hilecop.Sitpn.SitpnWellDefFired.
+
+(* Import lemmas on interpretation. *)
+
+Require Import Hilecop.Sitpn.SitpnWellDefInterpretation.
+
+(* Import lemmas on marking. *)
+
+Require Import Hilecop.Sitpn.SitpnRisingEdgeMarking.
+
+(* Import lemmas on well-definition. *)
+
+Require Import Hilecop.Sitpn.SitpnRisingEdgeWellDef.
+
+(* Import misc. tactics and lemmas. *)
+
+Require Import Hilecop.Utils.HilecopLemmas.
+Require Import Hilecop.Sitpn.SitpnTactics.
+
+(** * [sitpn_rising_edge] and [sitpn_state_eq] relation. *)
+
+(** ** [sitpn_state_eq], [sitpn_rising_edge] and marking. *)
+
+Lemma sitpn_rising_edge_state_eq_perm_marking :
+  forall (sitpn : Sitpn)
+         (s s' state state' : SitpnState),
+    IsWellDefinedSitpn sitpn ->
+    IsWellDefinedSitpnState sitpn s ->
+    IsWellDefinedSitpnState sitpn state ->
+    sitpn_state_eq s state ->
+    sitpn_rising_edge sitpn s = Some s' ->
+    sitpn_rising_edge sitpn state = Some state' ->
+    Permutation (marking s') (marking state').
+Proof.
+  intros sitpn s s' state state' Hwell_def_sitpn Hwell_def_s
+         Hwell_def_state Hsteq_sstate Hrising_s Hrising_state.
+
+  (* Stategy is to apply NoDup_Permutation, then we need: 
+     - NoDup (marking s')
+     - NoDup (marking state')
+     - ∀(p, n) ∈ (marking s') ⇔ (p, n) (marking state'). *)
+
+  (* Builds NoDup (marking s') and NoDup (marking state') *)
+  specialize (sitpn_rising_edge_well_def_state
+                sitpn s s' Hwell_def_sitpn Hwell_def_s Hrising_s)
+    as Hwell_def_s'.  
+  deduce_nodup_state_marking for s'.
+
+  specialize (sitpn_rising_edge_well_def_state
+                sitpn state state' Hwell_def_sitpn Hwell_def_state Hrising_state)
+    as Hwell_def_state'.
+  deduce_nodup_state_marking for state'.
+
+  rename Hnodup_fs_ms into Hnodup_ms.
+  rename Hnodup_fs_ms0 into Hnodup_mstate.
+
+  apply nodup_fst_split in Hnodup_ms.
+  apply nodup_fst_split in Hnodup_mstate.
+  
+  (* Specializes sitpn_rising_edge_sub_pre_add_post for 
+     Hrising_s and Hrising_state. *)
+  specialize (sitpn_rising_edge_sub_pre_add_post
+                sitpn s s' Hwell_def_sitpn Hwell_def_s Hrising_s)
+    as Hdef_marking_s'.
+  specialize (sitpn_rising_edge_sub_pre_add_post
+                sitpn state state' Hwell_def_sitpn Hwell_def_state Hrising_state)
+    as Hdef_marking_state'.
+Admitted.
+  
+(** ** [sitpn_state_eq], [sitpn_rising_edge] and action states. *)
+
+Lemma sitpn_rising_edge_state_eq_perm_actions :
+  forall (sitpn : Sitpn)
+         (s s' state state' : SitpnState),
+    IsWellDefinedSitpn sitpn ->
+    IsWellDefinedSitpnState sitpn s ->
+    IsWellDefinedSitpnState sitpn state ->
+    sitpn_state_eq s state ->
+    sitpn_rising_edge sitpn s = Some s' ->
+    sitpn_rising_edge sitpn state = Some state' ->
+    Permutation (exec_a s') (exec_a state').
+Proof.
+  intros sitpn s s' state state' Hwell_def_sitpn Hwell_def_s
+         Hwell_def_state Hsteq_sstate Hrising_s Hrising_state.
+
+  (* Specializes sitpn_rising_edge_same_actions for 
+     Hrising_s and Hrising_state. *)
+  specialize (sitpn_rising_edge_same_actions sitpn s s' Hrising_s)
+    as Heq_actions_s.
+  specialize (sitpn_rising_edge_same_actions sitpn state state' Hrising_state)
+    as Heq_actions_state.
+
+  (* Decomposes sitpn_state_eq s state to 
+     get Permutation (cond_values s) (cond_values state) *)
+  unfold sitpn_state_eq in Hsteq_sstate.
+  do 5 (apply proj2 in Hsteq_sstate).
+  specialize (proj1 Hsteq_sstate) as Hperm_actions.
+
+  (* Rewrites the goal and concludes. *)
+  rewrite Heq_actions_s, Heq_actions_state in Hperm_actions; assumption.
+Qed.
+
+(** ** [sitpn_state_eq], [sitpn_rising_edge] and condition values. *)
+
+Lemma sitpn_rising_edge_state_eq_perm_condv :
+  forall (sitpn : Sitpn)
+         (s s' state state' : SitpnState),
+    IsWellDefinedSitpn sitpn ->
+    IsWellDefinedSitpnState sitpn s ->
+    IsWellDefinedSitpnState sitpn state ->
+    sitpn_state_eq s state ->
+    sitpn_rising_edge sitpn s = Some s' ->
+    sitpn_rising_edge sitpn state = Some state' ->
+    Permutation (cond_values s') (cond_values state').
+Proof.
+  intros sitpn s s' state state' Hwell_def_sitpn Hwell_def_s
+         Hwell_def_state Hsteq_sstate Hrising_s Hrising_state.
+
+  (* Specializes sitpn_rising_edge_same_condv for 
+     Hrising_s and Hrising_state. *)
+  specialize (sitpn_rising_edge_same_condv sitpn s s' Hrising_s)
+    as Heq_condv_s.
+  specialize (sitpn_rising_edge_same_condv sitpn state state' Hrising_state)
+    as Heq_condv_state.
+
+  (* Decomposes sitpn_state_eq s state to 
+     get Permutation (cond_values s) (cond_values state) *)
+  unfold sitpn_state_eq in Hsteq_sstate.
+  do 4 (apply proj2 in Hsteq_sstate).
+  specialize (proj1 Hsteq_sstate) as Hperm_condv.
+
+  (* Rewrites the goal and concludes. *)
+  rewrite Heq_condv_s, Heq_condv_state in Hperm_condv; assumption.
+Qed.
+
+(** ** [sitpn_state_eq], [sitpn_rising_edge] and fired transitions. *)
+
+Lemma sitpn_rising_edge_state_eq_perm_fired :
+  forall (sitpn : Sitpn)
+         (s s' state state' : SitpnState),
+    IsWellDefinedSitpn sitpn ->
+    IsWellDefinedSitpnState sitpn s ->
+    IsWellDefinedSitpnState sitpn state ->
+    sitpn_state_eq s state ->
+    sitpn_rising_edge sitpn s = Some s' ->
+    sitpn_rising_edge sitpn state = Some state' ->
+    Permutation (fired s') (fired state').
+Proof.
+  intros sitpn s s' state state' Hwell_def_sitpn Hwell_def_s
+         Hwell_def_state Hsteq_sstate Hrising_s Hrising_state.
+
+  (* Specializes sitpn_rising_edge_same_fired for 
+     Hrising_s and Hrising_state. *)
+  specialize (sitpn_rising_edge_same_fired sitpn s s' Hrising_s)
+    as Heq_fired_s.
+  specialize (sitpn_rising_edge_same_fired sitpn state state' Hrising_state)
+    as Heq_fired_state.
+
+  (* Decomposes sitpn_state_eq s state to 
+     get Permutation (fired s) (fired state) *)
+  unfold sitpn_state_eq in Hsteq_sstate.
+  specialize (proj1 (proj2 Hsteq_sstate)) as Hperm_fired. 
+
+  (* Rewrites the goal and concludes. *)
+  rewrite Heq_fired_s, Heq_fired_state in Hperm_fired; assumption.
+Qed.
+  
+(** ** [sitpn_rising_edge] and [sitpn_state_eq]. *)
+
+Lemma sitpn_rising_edge_state_eq :
+  forall (sitpn : Sitpn)
+         (s s' state state' : SitpnState),
+    IsWellDefinedSitpn sitpn ->
+    IsWellDefinedSitpnState sitpn s ->
+    IsWellDefinedSitpnState sitpn state ->
+    sitpn_state_eq s state ->
+    sitpn_rising_edge sitpn s = Some s' ->
+    sitpn_rising_edge sitpn state = Some state' ->
+    sitpn_state_eq s' state'.
+Proof.
+  intros sitpn s s' state state' Hwell_def_sitpn Hwell_def_s
+         Hwell_def_state Hsteq_sstate Hrising_s Hrising_state.
+  unfold sitpn_state_eq.
+  repeat split.
+
+  (* CASE Permutation (marking s') (marking state') *)
+  - admit.
+
+  (* CASE Permutation (fired s') (fired state') *)
+  - apply (sitpn_rising_edge_state_eq_perm_fired
+             sitpn s s' state state' Hwell_def_sitpn Hwell_def_s
+             Hwell_def_state Hsteq_sstate Hrising_s Hrising_state).
+
+  (* CASE Permutation (d_intervals s') (d_intervals state') *)
+  - admit.
+
+  (* CASE Permutation (reset s') (reset state') *)
+  - admit.
+
+  (* CASE (cond_values s') (cond_values state') *)
+  - apply (sitpn_rising_edge_state_eq_perm_condv
+             sitpn s s' state state' Hwell_def_sitpn Hwell_def_s
+             Hwell_def_state Hsteq_sstate Hrising_s Hrising_state).
+
+  (* CASE (exec_a s') (exec_a state') *)
+  - apply (sitpn_rising_edge_state_eq_perm_actions
+             sitpn s s' state state' Hwell_def_sitpn Hwell_def_s
+             Hwell_def_state Hsteq_sstate Hrising_s Hrising_state).
+
+  (* CASE (exec_f s') (exec_f state') *)
+  - admit.
+Admitted.
